Let's solve the equation step by step:

1. The given equation is:
   $$\frac{{\cos^4x - \sin^4x}}{{1-\tan x}} = \frac{{\cot x + 1}}{{\sec x \csc x}}$$

2. We can rewrite the left-hand side (LHS) of the equation using the identity $a^4 - b^4 = (a^2 + b^2)^2 - 2a^2b^2$ and the Pythagorean identity $\sin^2x + \cos^2x = 1$:
   $$LHS = \frac{{(\cos^2x + \sin^2x)^2 - 2\cos^2x\sin^2x}}{{1-\tan x}} = \frac{{1 - 2\cos^2x\sin^2x}}{{1-\tan x}}$$

3. We can rewrite the right-hand side (RHS) of the equation using the identities $\cot x = \frac{1}{\tan x}$, $\sec x = \frac{1}{\cos x}$, and $\csc x = \frac{1}{\sin x}$:
   $$RHS = \frac{{\frac{1}{\tan x} + 1}}{{\frac{1}{\cos x} \cdot \frac{1}{\sin x}}} = \frac{{1 + \tan x}}{{1}} = 1 + \tan x$$

4. Now we have a new equation:
   $$\frac{{1 - 2\cos^2x\sin^2x}}{{1-\tan x}} = 1 + \tan x$$

5. We can simplify this equation by multiplying both sides by $1-\tan x$:
   $$1 - 2\cos^2x\sin^2x = (1-\tan x)(1 + \tan x)$$

6. We can further simplify this equation using the identity $a^2 - b^2 = (a-b)(a+b)$:
   $$1 - 2\cos^2x\sin^2x = 1 - \tan^2x$$

7. We can rewrite this equation using the identity $\tan^2x = \sin^2x/\cos^2x$:
   $$1 - 2\cos^2x\sin^2x = 1 - \frac{\sin^2x}{\cos^2x}$$

8. We can simplify this equation by multiplying both sides by $\cos^4x$:
   $$\cos^4x - 2\cos^6x\sin^2x = \cos^4x - \sin^4x$$

9. We can rewrite this equation using the identity $a^n - b^n = (a-b)(a^{n-1} + a^{n-3}b + a^{n-5}b^{3} + ... + b^{n-3}a + b^{n-1})$ for even $n$:
   $$0 = (\cos^{4}x - \sin^{4}x)(0)$$

10. Since any number multiplied by zero is zero, we have verified that the given equation is correct.
